Source/DafnyStandardLibraries/src/DafnyStdLibs/TargetSpecific/Concurrent-js.dfy
@@ -1,6 +1,68 @@
-module DafnyStdLibs.Concurrent refines ConcurrentInterface {
 
-  class MutableMap<K(==), V(==)> ... {
+module {:extern} {:compile false} DafnyStdLibs.Concurrent refines ConcurrentInterface {
+
+  class {:extern} MutableMap<K(==), V(==)> ... {
+
+    constructor {:extern} {:axiom} (ghost inv: (K, V) -> bool)
+      ensures this.inv == inv
+
+    ghost predicate Valid()
+    {
+      true
+    }
+
+    method {:extern} {:axiom} Keys() returns (keys: set<K>)
+
+    method {:extern} {:axiom} HasKey(k: K) returns (used: bool)
+
+    method {:extern} {:axiom} Values() returns (values: set<V>)
+
+    method {:extern} {:axiom} Items() returns (items: set<(K,V)>)
+
+    method {:extern} {:axiom} Put(k: K, v: V)
+
+    method {:extern} {:axiom} Get(k: K) returns (r: Option<V>)
+
+    method {:extern} {:axiom} Remove(k: K)
+
+    method {:extern} {:axiom} Size() returns (c: nat)
+
+  }
+
+  class {:extern} AtomicBox<T> ... {
+
+    constructor {:extern} {:axiom} (ghost inv: T -> bool, t: T)
+      requires inv(t)
+      ensures this.inv == inv
+
+    ghost predicate Valid() { true }
+
+    method {:extern} {:axiom} Get() returns (t: T)
+
+    method {:extern} {:axiom} Put(t: T)
+
+  }
+
+  class {:extern} Lock ... {
+
+    constructor {:extern} {:axiom} ()
+
+    method {:extern} {:axiom} Lock()
+
+    method {:extern} {:axiom} Unlock()
+
+  }
+}
+
+module DafnyStdLibs.ConcurrentDafny {
+
+  import opened Wrappers
+
+  class MutableMap<K(==), V(==)> {
+    
+    ghost const inv: (K, V) -> bool
+    ghost var knownKeys: set<K>
+    ghost var knownValues: set<V>
 
     var internal: map<K, V>
 
@@ -21,39 +83,55 @@ module DafnyStdLibs.Concurrent refines ConcurrentInterface {
     }
 
     ghost predicate Valid()
+      reads this
     {
       forall k :: k in internal.Keys ==> inv(k, internal[k]) && Contained()
     }
 
     method Keys() returns (keys: set<K>)
+      requires Valid()
+      ensures forall k :: k in keys ==> exists v :: v in knownValues && inv(k,v)
     {
       reveal Contained();
       keys := internal.Keys;
     }
 
     method HasKey(k: K) returns (used: bool)
+      requires Valid()
+      ensures used ==> exists v :: v in knownValues && inv(k,v)
     {
       reveal Contained();
       used := k in internal.Keys;
     }
 
     method Values() returns (values: set<V>)
+      requires Valid()
+      ensures forall v :: v in values ==> exists k :: k in knownKeys && inv(k,v)
     {
       reveal Contained();
       values := internal.Values;
     }
 
     method Items() returns (items: set<(K,V)>)
+      requires Valid()
+      ensures forall t :: t in items ==> inv(t.0, t.1)
     {
       items := internal.Items;
     }
 
     method Get(k: K) returns (r: Option<V>)
+      requires Valid()
+      ensures r.Some? ==> inv(k, r.value)
     {
       r := if k in internal.Keys then Some(internal[k]) else None;
     }
 
     method Put(k: K, v: V)
+      requires Valid()
+      requires inv(k, v)
+      modifies this
+      ensures Valid()
+
     {
       internal := internal[k := v];
       knownKeys := knownKeys + {k};
@@ -62,6 +140,10 @@ module DafnyStdLibs.Concurrent refines ConcurrentInterface {
     }
 
     method Remove(k: K)
+      requires Valid()
+      requires exists v :: inv(k,v)
+      modifies this
+      ensures Valid()
     {
       // only here to mollify the auditor
       assert exists v :: inv(k,v);
@@ -71,6 +153,7 @@ module DafnyStdLibs.Concurrent refines ConcurrentInterface {
     }
 
     method Size() returns (c: nat)
+      requires Valid()
     {
       // only here to mollify the auditor
       reveal Contained();
@@ -81,7 +164,10 @@ module DafnyStdLibs.Concurrent refines ConcurrentInterface {
 
   }
 
-  class AtomicBox<T> ... {
+  class AtomicBox<T> {
+
+    ghost const inv: T -> bool
+
     var boxed: T
 
     constructor (inv: T -> bool, t: T)
@@ -94,17 +180,21 @@ module DafnyStdLibs.Concurrent refines ConcurrentInterface {
     }
 
     ghost predicate Valid()
+      reads this
     {
       inv(boxed)
     }
 
     method Get() returns (t: T)
+      requires Valid()
       ensures inv(t)
     {
       t := boxed;
     }
 
     method Put(t: T)
+      requires inv(t)
+      modifies this
       ensures Valid()
     {
       boxed := t;
@@ -112,19 +202,29 @@ module DafnyStdLibs.Concurrent refines ConcurrentInterface {
 
   }
 
-  class Lock ... {
+  class Lock {
+
+    ghost var isLocked: bool
 
     constructor() {
       isLocked := false;
     }
 
-    method Lock() {
+    method Lock() 
+      requires !isLocked
+      modifies this
+      ensures isLocked
+    {
       // Written this way so that we don't get a warning about
       // "requires !isLocked" being an unnecessary precondition.
       isLocked := !isLocked;
     }
 
-    method Unlock() {
+    method Unlock() 
+      requires isLocked
+      modifies this
+      ensures !isLocked
+    {
       // Written this way so that we don't get a warning about
       // "requires isLocked" being an unnecessary precondition.
       isLocked := !isLocked;
